minor revisions to Seq and Map modules during recent development.

src/ghost/map.fst
@@ -17,25 +17,21 @@
 
 module Tesseract.Ghost.Map
 
-   type map 'key 'value = 
-      { 
-         maybe_lookup: 'key -> Tot (option 'value)
-      }
+   type map =
+      fun (key_t: Type) (val_t: Type) ->
+         key_t -> Tot (option val_t)
 
-   val empty: #key_t: Type -> #val_t: Type -> map key_t val_t
+   val empty: #key_t: Type -> #val_t: Type -> Tot (map key_t val_t)
    let empty (key_t: Type) (val_t: Type) = 
-      {
-         maybe_lookup = (fun (k: key_t) -> (None <: option val_t))
-      }
-
-   let maybe_lookup m = m.maybe_lookup
+      fun _ -> 
+         None
 
    val mem: #key_t: Type -> #val_t: Type -> map key_t val_t -> key_t -> Tot bool
-   let mem m k = is_Some (maybe_lookup m k)
+   let mem m k = is_Some (m k)
 
    val lookup: #key_t: Type -> #val_t: Type -> m: map key_t val_t -> k: key_t{mem m k} -> Tot val_t
    let lookup m k = 
-      match maybe_lookup m k with
+      match m k with
          | Some v ->
             v
 
@@ -43,10 +39,20 @@ module Tesseract.Ghost.Map
    let domain m = 
       Set.arbitrary (mem m)
 
-   val arbitrary: #key_t: Type -> #val_t: Type -> (key_t -> Tot (option val_t)) -> Tot (map key_t val_t)
-   let arbitrary fn =
-      {
-         maybe_lookup = fn
-      }
+   val update: #key_t: Type -> #val_t: Type -> map key_t val_t -> key_t -> val_t -> Tot (map key_t val_t)
+   let update (key_t: Type) (val_t: Type) m k v =
+      (fun kk ->
+         if k = kk then
+            Some v
+         else
+            m kk)
+
+   val add: #key_t: Type -> #val_t: Type -> m: map key_t val_t -> k: key_t{not (mem m k)} -> val_t -> Tot (map key_t val_t)
+   let add (key_t: Type) (val_t: Type) m k v =
+      update m k v
+
+   val subst: #key_t: Type -> #val_t: Type -> m: map key_t val_t -> k: key_t{mem m k} -> val_t -> Tot (map key_t val_t)
+   let subst (key_t: Type) (val_t: Type) m k v =
+      update m k v
 
 // $vim-fst:32: vim:set sts=3 sw=3 et ft=fstar:,$
